<?xml version="1.0" encoding="UTF-8"?>

<section xml:id="sec-factoring-and-graphing-polynomials" xmlns:xi="http://www.w3.org/2001/XInclude">
  <title>Factoring and Graphing Polynomials</title>
  
  <!-- <introduction>
  <p>
  This is the introduction to the section. It can contain any content
  that is valid in a <introduction> element, including <p>, <ul>, <ol>,
  <figure>, and <table>. You can also include other files using
  <xi:include> tags.
  </p>
  </introduction> -->
  
  <subsection>
    <title>Finding Roots of a Polynomial (Factoring Completely) Examples</title>
    
    <project>
      <title>Factoring Polynomials Examples</title>
      <introduction>
        <p>Find the roots of each polynomial function by factoring completely.</p>
      </introduction>
      <task>
        <statement><m>f(x) = x^3-3x^2-x+3</m>.</statement>
        <answer><m>f(x) = (x-1)(x-3)(x+1), x=-1,1,3</m>.</answer>
      </task>
      <task>
        <statement><m>f(x) = x^3+2x^2-5x-6</m>.</statement>
        <answer><m>f(x) = (x+1)(x-2)(x+3), x=-3,-1,2</m>.</answer>
      </task>
      <task>
        <statement><m>f(x) = x^4 + x^3 - 13x^2 - 25x - 12</m>.</statement>
        <answer><m>f(x) = (x+1)^2(x-4)(x+3), x=-1,4,-3</m>.</answer>
      </task>
      <task>
        <statement><m>f(x) = 2x^3-5x^2-4x+3</m>.</statement>
        <answer><m>f(x) = (x+1)(2x-1)(x-3), x=-1,\frac{1}{2},3</m>.</answer>
      </task>
      <task>
        <statement><m>f(x) = x^3 + 5x^2 + 2x - 8</m>.</statement>
        <answer><m>f(x) = (x-1)(x+2)(x+4), x=1,-2,-4</m>.</answer>
      </task>
      <task>
        <statement><m>f(x) = 2x^3-15x^2+22x+15</m>.</statement>
        <answer><m>f(x) = (x-3)(2x+1)(x-5), x=3,-\frac{1}{2},5</m>.</answer>
      </task>
      <task>
        <statement><m>f(x) = -x^3 - x^2 + 22x + 40</m>.</statement>
        <answer><m>f(x) = -(x+2)(x+4)(x-5), x=-2,-4,5</m>.</answer>
      </task>
      <task>
        <statement><m>f(x) = 3x^3 - 4x^2 - 59x + 20</m>.</statement>
        <answer><m>f(x) = (x+4)(x-5)(3x-1), x=-4,5,\frac{1}{3}</m>.</answer>
      </task>
      <task>
        <statement><m>f(x) = 3x^3 - 4x^2 - 5x + 2</m>.</statement>
        <answer><m>f(x) = (x+1)(x-2)(3x-1), x=-1,2,\frac{1}{3}</m>.</answer>
      </task>
      <task>
        <statement><m>f(x) = x^4-5x^3+2x^2+20x-24</m>.</statement>
        <answer><m>f(x) = (x-2)^2(x+2)(x-3), x=2,-2,3</m>.</answer>
      </task>
      <task>
        <statement><m>f(x) = x^4-3x^3-7x^2+15x+18</m>.</statement>
        <answer><m>f(x) = (x+1)(x+2)(x-3)^2, x=-1,-2,3</m>.</answer>
      </task>
      <task>
        <statement><m>f(x)=x^3-6x^2+11x-6</m>.</statement>
        <answer><m>f(x)=(x-1)(x-2)(x-3), x=1,2,3</m>.</answer>
      </task>
      <task>
        <statement><m>f(x)=x^3+3x^2-4</m>.</statement>
        <answer><m>f(x)=(x-1)(x+2)^2, x=1,-2</m>.</answer>
      </task>
      <task>
        <statement><m>f(x)=x^3+2x^2-x-2</m>.</statement>
        <answer><m>f(x)=(x-1)(x+1)(x+2), x=-2,-1,1</m>.</answer>
      </task>
      <task>
        <statement><m>f(x)=x^3+x^2-16x-16</m>.</statement>
        <answer><m>f(x)=(x-4)(x+1)(x+4), x=-4,-1,4</m>.</answer>
      </task>
      <task>
        <statement><m>f(x)=x^4+4x^3-7x^2-34x-24</m>.</statement>
        <answer><m>f(x)=(x-3)(x+1)(x+2)(x+4), x=-4,-2,-1,3</m>.</answer>
      </task>
      <task>
        <statement><m>f(x)=3x^3 + x^2 - 20x + 12</m>.</statement>
        <answer><m>f(x)=(x-2)(x+3)(3x-2), x=2,-3,\frac{2}{3}</m>.</answer>
      </task>
      <task>
        <statement><m>f(x)=x^5+3x^4-5x^3-15x^2+4x+12</m>.</statement>
        <answer><m>f(x)=(x-2)(x-1)(x+1)(x+2)(x+3), x=-3,-2,-1,1,2</m>.</answer>
      </task>
      <task>
        <statement><m>f(x)=x^4-4x^2</m>.</statement>
        <answer><m>f(x) = x^2(x-2)(x+2), x=0,2,-2</m>.</answer>
      </task>
      <task>
        <statement><m>f(x)=x^5+3x^4-x^3-7x^2 + 4</m>.</statement>
        <answer><m>f(x)=(x-1)^2(x+1)(x+2)^2, x=-2,-1,1</m>.</answer>
      </task>
      <task>
        <statement><m>f(x)=x^3-2x^2-9x+18</m>.</statement>
        <answer><m>f(x)=(x-3)(x-2)(x+3), x=-3,2,3</m>.</answer>
      </task>
      <task>
        <statement><m>f(x) = x^3 + 7x^2 + 16x + 12</m>.</statement>
        <answer><m>f(x) = (x+2)^2(x+3), x=-3,-2</m>.</answer>
      </task>
      <task>
        <statement><m>f(x)=x^3-7x^2+7x+15</m>.</statement>
        <answer><m>f(x)=(x-5)(x-3)(x+1), x=5,3,-1</m>.</answer>
      </task>
      <task>
        <statement><m>f(x)=x^3-7x^2-41x-33</m>.</statement>
        <answer><m>f(x)=(x-11)(x+1)(x+3), x=11,-1,-3</m>.</answer>
      </task>
      <task>
        <statement><m>f(x)=x^4+2x^3-7x^2-8x+12</m>.</statement>
        <answer><m>f(x)=(x-2)(x-1)(x+2)(x+3), x=2,1,-2,-3</m>.</answer>
      </task>
      <task>
        <statement><m>f(x) = x^3 - 4x^2 - 45x</m>.</statement>
        <answer><m>f(x) = x(x - 9)(x + 5), x=0,9,-5</m>.</answer>
      </task>
      <task>
        <statement><m>f(x) = x^4 - 81x^2</m>.</statement>
        <answer><m>f(x) = x^2(x - 9)(x + 9), x=0,9,-9</m>.</answer>
      </task>
      <task>
        <statement><m>f(x) = x^3 + 3x^2 - x - 3</m>.</statement>
        <answer><m>f(x) = (x - 1)(x + 1)(x + 3), x=1,-1,-3</m>.</answer>
      </task>
      <task>
        <statement><m>f(x) = -x^4 - 2x^3 + 7x^2 + 8x - 12</m>.</statement>
        <answer><m>f(x) = -(x - 2)(x - 1)(x + 2)(x + 3), x=2,1,-2,-3</m>.</answer>
      </task>
      <task>
        <statement><m>f(x) = x^4 - 4x^3 + x^2 + 6x</m>.</statement>
        <answer><m>f(x) = x(x - 3)(x - 2)(x + 1), x=0,3,2,-1</m>.</answer>
      </task>
      <task>
        <statement><m>f(x) = x^3 + 3x^2 - 6x - 8</m>.</statement>
        <answer><m>f(x) = (x - 2)(x + 1)(x + 4), x=2,-1,-4</m>.</answer>
      </task>
      <task>
        <statement><m>f(x) = x^3 - 4x^2 + x + 6</m>.</statement>
        <answer><m>f(x) = (x - 3)(x - 2)(x + 1), x=3,2,-1</m>.</answer>
      </task>
      <task>
        <statement><m>f(x) = -x^3 + 5x^2 - 7x + 3</m>.</statement>
        <answer><m>f(x) = -(x - 3)(x - 1)^2, x=3,1</m>.</answer>
      </task>
      <task>
        <statement><m>f(x) = -x^4 - 2x^3 + 3x^2 + 4x - 4</m>.</statement>
        <answer><m>f(x) = -(x - 1)^2(x + 2)^2, x=1,-2</m>.</answer>
      </task>
    </project>
    
    <project>
      <title>Examples with irrational roots or irreducible quadratic factors</title>
      <introduction>
        <p>Find the roots of each polynomial function by factoring completely.</p>
      </introduction>
      <task>
        <statement><m>f(x)=x^5 - 3x^4 + 8x^2 - 9x + 3</m>.</statement>
        <answer><m>f(x)=(x-1)^3(x^2-3), x=1, \sqrt{3}, -\sqrt{3}</m>.</answer>
      </task>
      <task>
        <statement><m>f(x)=x^3-27x+10</m>.</statement>
        <answer><m>f(x)=(x-5)(x^2+5x-2), x=5, x=\frac{-5\pm\sqrt{33}}{2}</m>.</answer>
      </task>
      <task>
        <statement><m>f(x)=x^4+5x^3+2x^2+7x-15</m>.</statement>
        <answer><m>f(x)=(x-1)(x+5)(x^2+x+3), x=1,-5</m>.</answer>
      </task>
      <task>
        <statement><m>f(x) = 2x^3 - 8x^2 - x + 4</m>.</statement>
        <answer><m>f(x) = (x-4)(2x^2-1), x = 4, \pm \frac{1}{\sqrt{2}}</m>.</answer>
      </task>
      <task>
        <statement><m>f(x)=x^4+9x^3+12x^2-11x+21</m>.</statement>
        <answer><m>f(x)=(x+3)(x+7)(x^2-x+1), x=-3,-7</m>.</answer>
      </task>
      <task>
        <statement><m>f(x)=3x^3+5x^2-3x-2</m>.</statement>
        <answer><m>f(x)=(x+2)(3x^2-x-1), x=-2, \frac{1\pm\sqrt{13}}{6}</m>.</answer>
      </task>
      <task>
        <statement><m>f(x) = -2x^4 + 4x^3 + 15x^2 - 16x - 28</m>.</statement>
        <answer><m>f(x) = (x-2)(x+2)(-2x^2 + 4x + 7), x = 2, -2, \frac{2 \pm 3\sqrt{2}}{2}</m>.</answer>
      </task>
    </project>
  </subsection>
  
  <subsection xml:id="summary-of-factoring-polynomials">
    <title>Summary of Factoring Higher-Degree Polynomial Functions</title>
    <ol>
      <li>
        <p>(If necessary) Write the polynomial in descending power order.</p>
      </li>
      <li>
        <p>
          Check for common factors. If there are any common factors, either a variable, number, or both. If so, factor out the greatest common factor (GCF).
        </p>
        <ul>
          <li>e.g. <m>f(x) = 6x^3 - 12x^2 + 18x = 6x(x^2-2x+3)</m>.</li>
          <li>e.g. <m>f(x) = x^4 - 2x^3 - 11x^2 + 12x = x(x^3-2x^2-11x+12)</m>.</li>
          <li>If the leading coefficient is negative, factor out <m>-1</m> from all its terms.</li>
          <li>Especially check if the numbers in the equation are big!</li>
        </ul>
      </li>
      <li>
        <p>
          Find one factor, by testing potential zeros until you find a zero. If <m>x = a</m> is a zero, then <m>x-a</m> is a factor (factor theorem).
        </p>
        <ul>
          <li>Can find zeros using your scientific calculator (if allowed) with TABLE mode.</li>
        </ul>
        <p>
          List all of the potential roots to show your work (if required).
        </p>
        <ul>
          <li>If the leading coefficient is 1, then all potential integer roots are the factors of the constant term (integral zero theorem).</li>
          <li>
            <p>
              If the leading coefficient is not 1, then the possible roots are all fractions of the form <m>\frac{p}{q}</m>, where:
            </p>
            <ul>
              <li><m>p</m> is a factor of the constant term</li>
              <li><m>q</m> is a factor of the leading coefficient</li>
            </ul>
            <p>
              (rational root theorem)
            </p>
          </li>
        </ul>
      </li>
      <li>
        <p>Divide out the factor, using synthetic division, so that the resulting polynomial has a degree 1 lower than originally.</p>
      </li>
      <li>
        <p>
          Repeat the steps, until the resulting polynomial is quadratic.
        </p>
        <ul>
          <li>You can stack multiple synthetic divisions together for conciseness.</li>
          <li>If <m>x=a</m> is a zero, it could still be a zero again (if it is a repeated zero).</li>
        </ul>
      </li>
      <li>
        <p>Factor the quadratic. If it's not factorable, use the quadratic formula to check for potential irrational zeros.</p>
      </li>
    </ol>
    <p>
      Note: Also keep in mind other special factoring patterns, which can sometimes be used instead of synthetic divison:
    </p>
    <ul>
      <li>
        <p>
          Difference of squares, sum of cubes, difference of cubes.
        </p>
        <md>
          <mrow>a^2 - b^2 \amp = (a + b)(a - b) \amp x^2 - 9 \amp= (x+3)(x-3)</mrow>
          <mrow>a^3 + b^3 \amp = (a + b)(a^2 - ab + b^2) \amp x^3 + 8 \amp= (x+2)(x^2 - 2x + 4)</mrow>
          <mrow>a^3 - b^3 \amp = (a - b)(a^2 + ab + b^2) \amp x^3 - 27 \amp= (x-3)(x^2+3x+9)</mrow>
        </md>
      </li>
      <li>
        <p>Quadratic form (e.g. <m>u = x^2</m> or <m>u = x^3</m>).</p>
      </li>
      <li>
        <p>Factor by grouping.</p>
      </li>
    </ul>
    
    <p>
      Some remarks:
    </p>
    <ul>
      <li>The order you find the factors doesn't really matter, in that any order will eventually lead you to the same final factored form. However, if testing zeros, it is often easier and more systematic to start from the simplest and smallest zeros, like 1 or <m>-1</m>, maybe 2 or <m>-2</m>, etc.</li>
      <li>If you test a number and it is a root, it can still be a root again for the reduced polynomial (if it is a multiple root). However, if you test it and it's not a root, then you can skip that for the reduced polynomial.</li>
    </ul>
  </subsection>
  
</section>