<?xml version="1.0" encoding="UTF-8"?>

<section xml:id="sec-factoring-quadratics-summary" xmlns:xi="http://www.w3.org/2001/XInclude">
  <title>Factoring Quadratics Summary</title>
  
  <introduction>
    <ol>
      <li>
        <p>
          Write the quadratic in descending power order (standard form), <m>ax^2 + bx + c</m>.
        </p>
        <p>
          <ul>
            <li>
              <p>
                e.g. <m>-5 - 4x + x^2 = x^2 - 4x - 5</m>
              </p>
            </li>
          </ul>
        </p>
      </li>
      <li>
        <p>
          If there is a GCF (greatest common factor), factor it out (either a number or variable like <m>x</m>).
        </p>
        <p>
          <ul>
            <li>
              <p>
                e.g. <m>x^2 + 4x = x(x+4)</m>
              </p>
            </li>
            <li>
              <p>
                e.g. <m>2x^2 + 4x - 6 = 2(x^2 + 2x - 3)</m>
              </p>
            </li>
          </ul>
        </p>
      </li>
      <li>
        <p>
          Determine which factoring method applies, based on the form:
        </p>
        <ol marker="(a)">
          <li>
            <p>
              If <m>a = 1</m>, find two numbers that multiply to <m>c</m> and add to <m>b</m>.
            </p>
            <p>
              <ul>
                <li>
                  <p>
                    e.g. <m>x^2 + 5x + 6 = (x+2)(x+3)</m>
                  </p>
                </li>
              </ul>
            </p>
          </li>
          <li>
            <p>
              If <m>a \neq 1</m>, use the cross method (or <m>ac</m>-method, or box method).
            </p>
            <p>
              <ul>
                <li>
                  <p>
                    e.g. <m>2x^2 + 7x + 3 = (2x+1)(x+3)</m>
                  </p>
                </li>
              </ul>
            </p>
          </li>
          <li>
            <p>
              If there are only 2 terms, try difference of squares.
            </p>
            <md>
              <mrow>
                a^2 - b^2 = (a+b)(a-b) \qquad \text{e.g. } x^2 - 9 = (x+3)(x-3)
              </mrow>
            </md>
          </li>
          <li>
            <p>
              (Optional) use perfect square factoring patterns:
            </p>
            <md>
              <mrow>
                \begin{aligned}
                a^2 + 2ab + b^2 \amp = (a+b)^2 \\
                a^2 - 2ab + b^2 \amp = (a-b)^2
                \end{aligned}
                \qquad
                \begin{aligned}
                \text{e.g. } x^2+6x+9 \amp = (x+3)^2 \\
                \text{e.g. } 4x^2 - 12x + 9 \amp = (2x-3)^2
                \end{aligned}
              </mrow>
            </md>
          </li>
        </ol>
      </li>
    </ol>
    
  </introduction>
  
  <subsection xml:id="factoring-flowchart">
    <title>Factoring Quadratics Flowchart</title>
    <image>
      <latex-image>
        \begin{tikzpicture}[
        node distance=0.8cm and 0.8cm, % tight spacing
        every node/.style={font=\small},
        line/.style={-Latex, shorten >=1pt},
        process/.style={rectangle,rounded corners,draw,align=center,inner sep=3pt,text width=6cm},
        decision/.style={diamond,draw,aspect=1.8,align=center,inner sep=2pt,text width=2.8cm},
        processNarrow/.style={rectangle,rounded corners,draw,align=left,inner sep=3pt,text width=5.6cm},
        processBottom/.style={rectangle,rounded corners,draw,align=left,inner sep=3pt,text width=6cm}
        ]
        % Top: standard form, then GCF
        \node[process] (order) {
          \makebox[\linewidth]{\textbf{Write in standard form}}\\[2pt]
          Write the quadratic with the \(x^2\) term first, then the \(x\) term, and the constant last (standard form \(ax^2+bx+c\)).\\
          \(\text{e.g. } -4x - 5 + x^2 = x^2 - 4x - 5\)
        };
        
        \node[decision,below=0.6cm of order] (gcfq) {\textbf{Is there a GCF?}};
        
        \node[processNarrow,below left=0.6cm and 1.2cm of gcfq] (gcfy) {
          \makebox[\linewidth]{\textbf{Factor out the GCF}}\\[2pt]
          (number or variable) \\
          \(\text{e.g. } x^2 + 4x = x(x+4)\)\\
          \(\text{e.g. } 2x^2 + 4x - 6 = 2(x^2 + 2x - 3)\)
        };
        
        % Terms decision
        \node[decision,below=1.1cm of gcfq] (terms) {\textbf{How many terms?}};
        
        % Bottom: two boxes (binomial vs trinomial)
        \node[processBottom,below left=1cm and -0.6cm of terms] (two) {%
          \makebox[\linewidth]{\textbf{Two terms (binomial)}}\\[2pt]
          Try \textbf{difference of squares} \\[2pt]
          \(a^2 - b^2 = (a+b)(a-b)\) \\
          \(\text{e.g. } x^2 - 9 = (x+3)(x-3)\)
        };
        
        \node[processBottom,below right=1cm and -0.6cm of terms] (three) {%
          \makebox[\linewidth]{\textbf{Three terms (trinomial)}}\\[2pt]
          \(\bullet\) If \(a=1\): find two numbers that multiply to \(c\) and add to \(b\).\\
          \(\quad\) \(\text{e.g. } x^2 + 5x + 6 = (x+2)(x+3)\)\\[3pt]
          \(\bullet\) If \(a\ne 1\): use the \textbf{cross method} (or \(ac\)-method, or box method).\\
          \(\quad\) \(\text{e.g. } 2x^2 + 7x + 3 = (2x+1)(x+3)\)\\[8pt]
          \(\bullet\) (Optional) Perfect square trinomials.\\
          \(a^2 + 2ab + b^2 = (a+b)^2\) \\
          \(a^2 - 2ab + b^2 = (a-b)^2\) \\
          \(\text{e.g. } x^2 + 6x + 9 = (x+3)^2\)\\
          \(\text{e.g. } 4x^2 - 12x + 9 = (2x-3)^2\)
        };
        
        % Arrows
        \draw[line] (order) -- (gcfq);
        \draw[line] (gcfq) -- node[midway,above left] {\textbf{Yes}} (gcfy);
        \draw[line] (gcfy.south) |- (terms.west);
        \draw[line] (gcfq) -- node[midway,right] {\textbf{No}} (terms);
        \draw[line] (terms) -- node[midway,above] {\textbf{2}} (two.north);
        \draw[line] (terms) -- node[midway,above] {\textbf{3}} (three.north);
        \end{tikzpicture}
      </latex-image>
    </image>
  </subsection>
  
  
  
</section>